src/promotion/SimThreadPromotion.v
@@ -90,37 +90,75 @@ Inductive sim_state_cas_fail (l: Loc.t) (r: Reg.t) (st_src st_tgt: State.t): Pro
 .
 Hint Constructors sim_state_cas_fail.
 
+Definition sim_state (l: Loc.t) (r: Reg.t) (st_src st_tgt: State.t): Prop :=
+  sim_state_promotion l r st_src st_tgt \/
+  sim_state_fa l r st_src st_tgt \/
+  sim_state_cas_success1 l r st_src st_tgt \/
+  sim_state_cas_success2 l r st_src st_tgt \/
+  sim_state_cas_fail l r st_src st_tgt
+.
+
 Inductive sim_thread_promotion (l: Loc.t) (r: Reg.t) (e_src e_tgt: Thread.t lang): Prop :=
 | sim_thread_promotion_intro
     (REGFREE: reg_free_stmts r e_src.(Thread.state).(State.stmts))
-    (STMTS: sim_state_promotion l r e_src.(Thread.state) e_tgt.(Thread.state) \/
-            sim_state_fa l r e_src.(Thread.state) e_tgt.(Thread.state) \/
-            sim_state_cas_success1 l r e_src.(Thread.state) e_tgt.(Thread.state) \/
-            sim_state_cas_success2 l r e_src.(Thread.state) e_tgt.(Thread.state) \/
-            sim_state_cas_fail l r e_src.(Thread.state) e_tgt.(Thread.state))
+    (STMTS: sim_state l r e_src.(Thread.state) e_tgt.(Thread.state))
     (LOCAL: sim_local l e_src.(Thread.local) e_tgt.(Thread.local))
     (SC: sim_timemap l e_src.(Thread.sc) e_tgt.(Thread.sc))
     (MEMORY: sim_memory l e_src.(Thread.memory) e_tgt.(Thread.memory))
     (LATEST: exists from released,
         Memory.get l (Memory.max_ts l e_src.(Thread.memory)) e_src.(Thread.memory) = 
         Some (from, Message.full (e_tgt.(Thread.state).(State.regs) r) released))
+    (PROMISES: forall to, Memory.get l to e_src.(Thread.local).(Local.promises) = None)
+    (RELEASED: forall loc from to val released
+                 (GETP: Memory.get loc to e_src.(Thread.local).(Local.promises) =
+                        Some (from, Message.full val (Some released))),
+        released_eq_tview_loc l loc released e_src.(Thread.local).(Local.tview))
 .
 Hint Constructors sim_thread_promotion.
 
 Inductive sim_thread_promotion_reserve (l: Loc.t) (r: Reg.t) (e_src e_tgt: Thread.t lang): Prop :=
 | sim_thread_promotion_reserve_intro
     (REGFREE: reg_free_stmts r e_src.(Thread.state).(State.stmts))
-    (STMTS: sim_state_promotion l r e_src.(Thread.state) e_tgt.(Thread.state) \/
-            sim_state_fa l r e_src.(Thread.state) e_tgt.(Thread.state) \/
-            sim_state_cas_success1 l r e_src.(Thread.state) e_tgt.(Thread.state) \/
-            sim_state_cas_success2 l r e_src.(Thread.state) e_tgt.(Thread.state) \/
-            sim_state_cas_fail l r e_src.(Thread.state) e_tgt.(Thread.state))
+    (STMTS: sim_state l r e_src.(Thread.state) e_tgt.(Thread.state))
     (LOCAL: sim_local l e_src.(Thread.local) e_tgt.(Thread.local))
     (SC: sim_timemap l e_src.(Thread.sc) e_tgt.(Thread.sc))
     (MEMORY: sim_memory l e_src.(Thread.memory) e_tgt.(Thread.memory))
     (LATEST: Memory.latest_val l e_src.(Thread.memory) (e_tgt.(Thread.state).(State.regs) r))
-    (RESERVE: exists from,
-        Memory.get l (Memory.max_ts l e_src.(Thread.memory)) e_src.(Thread.memory) = 
+    (PROMISES: forall to (TO: to <> Memory.max_ts l e_src.(Thread.memory)),
+        Memory.get l to e_src.(Thread.local).(Local.promises) = None)
+    (RELEASED: forall loc from to val released
+                 (GETP: Memory.get loc to e_src.(Thread.local).(Local.promises) =
+                        Some (from, Message.full val (Some released))),
+        released_eq_tview_loc l loc released e_src.(Thread.local).(Local.tview))
+    (MEM: exists from,
+        Memory.get l (Memory.max_ts l e_src.(Thread.memory)) e_src.(Thread.memory) =
+        Some (from, Message.reserve))
+    (PROMISE: exists from,
+        Memory.get l (Memory.max_ts l e_src.(Thread.memory)) e_src.(Thread.local).(Local.promises) = 
         Some (from, Message.reserve))
 .
 Hint Constructors sim_thread_promotion_reserve.
+
+Lemma step_sim_thread_promotion_reserve
+      l r e_src e_tgt
+      (SIM: sim_thread_promotion l r e_src e_tgt):
+  exists from to e1_src,
+    <<STEP: Thread.step false (ThreadEvent.promise l from to Message.reserve Memory.op_kind_add)
+                        e_src e1_src>> /\
+    <<SIM: sim_thread_promotion_reserve l r e1_src e_tgt>>.
+Proof.
+  destruct e_src, e_tgt. inv SIM. ss.
+  guardH STMTS. des.
+Admitted.
+
+Lemma step_sim_thread_promotion
+      l r e_src e_tgt
+      (SIM: sim_thread_promotion_reserve l r e_src e_tgt):
+  exists from to e1_src,
+    <<STEP: Thread.step false (ThreadEvent.promise l from to Message.reserve Memory.op_kind_cancel)
+                        e_src e1_src>> /\
+    <<SIM: sim_thread_promotion l r e1_src e_tgt>>.
+Proof.
+  destruct e_src, e_tgt. inv SIM. ss.
+  guardH STMTS. des.
+Admitted.
